*Recall [[Complex Number Exponential Form]]* and [[Eulers Formula]] $e^{i\theta} = cos(\theta) + isin(\theta)$ so $z = |z|e^{i\theta}$ . The same process follows as if we were [[Converting from Rectangular Form to Polar]] .

### Example 
___
*Suppose $z = 1 - \sqrt{3}i$* 

$|z| = \sqrt{(-1)^2 + (-\sqrt{3})^2}$
$|z| = \sqrt{1 + 3}$
$|z| = \sqrt{4}$
$|z| = 2$

Calculate Argument . 

$\theta = tan^{-1}(\frac{b}{a})$
$\theta = tan^{-1}(\frac{-\sqrt{3}}{1})$
### Example 
___

*Suppose $z = 4 - 4i$* 

$|z| = \sqrt{(4)^2 + (-{4})^2}$
$|z| = \sqrt{32}$
$|z| = \sqrt{4}$
$|z| = 2$

Calculate Argument . 

$\theta = tan^{-1}(\frac{b}{a})$
$\theta = tan^{-1}(\frac{-\sqrt{3}}{1})$
____

Tags : #math #linear-algebra
